new-backend/bvl_inlineScript.sml
@@ -61,9 +61,7 @@ val bEval_code_lemma = prove(
   \\ REPEAT (BasicProvers.FULL_CASE_TAC \\ FULL_SIMP_TAC (srw_ss()) [])
   \\ CONV_TAC (DEPTH_CONV PairRules.PBETA_CONV)
   \\ FULL_SIMP_TAC (srw_ss()) [dec_clock_def]
-  \\ POP_ASSUM MP_TAC \\ SIMP_TAC std_ss [bEvalOp_def]
-  \\ REPEAT (BasicProvers.FULL_CASE_TAC \\ FULL_SIMP_TAC (srw_ss()) [])
-  \\ REPEAT STRIP_TAC \\ FULL_SIMP_TAC std_ss []);
+  \\ IMP_RES_TAC bEvalOp_const \\ FULL_SIMP_TAC std_ss []);
 
 val bEval_code = store_thm("bEval_code",
   ``!xs env s1 vs s2. (bEval (xs,env,s1) = (vs,s2)) ==> (s2.code = s1.code)``,
